WIP try gen correctly

gen.thy
@@ -29,30 +29,98 @@ ML_file \<open>jclause.ML\<close>
 ML_file \<open>jeha_proof.ML\<close>
 ML_file \<open>jeha_unify.ML\<close>
 
-
-
+(* Antiquotations for term and type patterns from the cookbook. *)
 ML \<open>
-  open SpecCheck
-  open SpecCheck_Generator
+  val term_pat_setup =
+  let
+    val parser = Args.context -- Scan.lift Parse.embedded_inner_syntax
+
+    fun term_pat (ctxt, str) =
+      str |> Proof_Context.read_term_pattern ctxt |> ML_Syntax.print_term |> ML_Syntax.atomic
+  in
+    ML_Antiquotation.inline @{binding "term_pat"} (parser >> term_pat)
+  end
+
+  val type_pat_setup =
+  let
+    val parser = Args.context -- Scan.lift Parse.embedded_inner_syntax
+
+    fun typ_pat (ctxt, str) =
+      let
+        val ctxt' = Proof_Context.set_mode Proof_Context.mode_schematic ctxt
+      in
+        str |> Syntax.read_typ ctxt' |> ML_Syntax.print_typ |> ML_Syntax.atomic
+      end
+  in
+    ML_Antiquotation.inline @{binding "typ_pat"} (parser >> typ_pat)
+  end
 \<close>
 
+setup \<open> term_pat_setup \<close>
+
+setup \<open> type_pat_setup \<close>
+
 ML \<open>
+  (* probability of generating a constant *)
+  val prob_of_constant = 0.3
   (* Precomputed, from the paper, presumably increasing the probability of
   boltzmann_index leads to smaller terms. Weaker effect when increasing the
   probability of boltzmann_lambda. *)
-  fun boltzmann_index r = r < 0.35700035696434995;
-  fun boltzmann_lambda r = r < 0.6525813160382378;
+  (* Scale precomputed values into interval determined by 1 - prob_of_constant. *)
+  fun rescale r = (1.0 - prob_of_constant) * r + prob_of_constant
+  fun boltzmann_constant r = r < prob_of_constant
+  fun boltzmann_index r = r < rescale 0.35700035696434995;
+  fun boltzmann_lambda r = r < rescale 0.6 (* 0.6525813160382378 *);
   (* The probability p of de Bruijn index 0, generally Bound j has the
   probability (1-p)^j * p (geometric distribution) *)
-  fun boltzmann_leaf r = r < 0.7044190409261122;
+  fun boltzmann_leaf r = r < rescale 0.65 (* 0.7044190409261122 *);
+\<close>
 
+ML \<open>
+  (* Adds unused additional state to a generator. Allows us to reuse existing generators. *)
+  val lift_gen : ('a, 's) SpecCheck_Gen_Types.gen_state -> ('a, 'b * 's) SpecCheck_Gen_Types.gen_state =
+    fn gen => (fn (b, s) => let val (a, s) = gen s in (a, (b, s)) end)
+  (* Like gen but with unification state. *)
+  type 'a unif_gen = ('a, (Proof.context * typ list * Type.tyenv * int * typ) * SpecCheck_Random.rand) SpecCheck_Gen_Types.gen_state
+  val fresh_type_indexname : indexname unif_gen =
+    fn ((ctxt, Ts, typ_env, maxidx, T), s) =>
+      ((Name.aT, maxidx), ((ctxt, Ts, typ_env, maxidx + 1, T), s))
+  val defaultS : sort unif_gen = fn (s as ((ctxt, _, _, _, _), _)) =>
+    (Sign.defaultS (Proof_Context.theory_of ctxt), s)
+  val fresh_tvar : typ unif_gen =
+    SpecCheck_Gen_Term.tvar
+      fresh_type_indexname
+      defaultS
+  (* Each term generator guarantees that it generates a term whose type unifies
+  with the type T in the type environment it returns (unless it fails). *)
+  (* FIXME: broken. We don't need to return Ts or T! But how? They depend on the state... *)
+  (*
+  fun bound ((_, [], _, _), _) = error "bound: not below lambda"
+    | bound ((ctxt, bT::bound_Ts, typ_env, maxidx, T), s) =
+        let val (r, s) = SpecCheck_Random.real_unit s in
+          if boltzmann_index r
+            then
+              let
+                val (typ_env, maxidx) = Sign.typ_unify (Proof_Context.theory_of ctxt) (bT, T) (typ_env, maxidx)
+              in
+                (Bound 0, ((ctxt, bT::bound_Ts, typ_env, maxidx, T), s))
+              end
+            else
+              (* FIXME: increase Bound, reset Ts *)
+              bound ((ctxt, bound_Ts, typ_env, maxidx, T), s)
+        end
+  *)
+  (* val abs : typ_unif_gen = *)
+\<close>
+
+ML \<open>
   (* (rng state, env, maxidx) *)
   type term_state = SpecCheck_Random.rand * Type.tyenv * int;
 
   fun pick_index _ [] _ _ = error "pick_index: not below lambda"
     | pick_index (ctxt : Proof.context) (T::Ts) typ (s, env) =
     let
-      val (r, s) = range_real (0.0, 1.0) s
+      val (r, s) = SpecCheck_Generator.range_real (0.0, 1.0) s
     in
       if boltzmann_leaf r
         then ((s, Sign.typ_unify (Proof_Context.theory_of ctxt) (T, typ) env), Bound 0)
@@ -64,6 +132,37 @@ ML \<open>
 
   fun gen_fresh_tyvar ctxt maxidx =
     (maxidx + 1, TVar ((Name.aT, maxidx + 1), Sign.defaultS (Proof_Context.theory_of ctxt)));
+  
+  fun ran_constant ctxt typ (s, (typ_env, maxidx)) =
+    let
+      fun upshift_TVar j (TVar ((name, i), T)) = TVar ((name, i + j), T)
+        | upshift_TVar _ T = T
+      fun map_const f (t as (Const _)) = f t
+        | map_const _ t = t
+      val freshen_type = map_const (map_types (map_atyps (upshift_TVar maxidx)))
+      val constants =
+        ctxt
+        |> Proof_Context.theory_of
+        |> Sign.consts_of
+        |> Consts.dest
+        |> #constants
+        (* discard Pure... constants, length of 11 is a good cutoff that includes HOL.False *)
+        |> filter (fn (name, _) => String.isPrefix "HOL" name andalso String.size name <= 11)
+        (* |> filter (fn (name, _) => String.isPrefix "HOL.All" name orelse String.isPrefix "HOL.False" name) *)
+        |> map (fn (name, (T, _)) => Const (name, T))
+        (* |> curry (op @) [Free ("c", TVar (("'a", 0), [])), Free ("d", TVar (("'b", 0), []))] *)
+      val (constant, s) = SpecCheck_Generator.elementsL constants s
+      val constant = freshen_type constant
+      val T = fastype_of constant
+      val maxidx = Term.maxidx_typ T maxidx
+      val (typ_env, maxidx) =
+        Sign.typ_unify
+          (Proof_Context.theory_of ctxt)
+          (T, typ)
+          (typ_env, maxidx)
+    in
+      ((s, (typ_env, maxidx)), constant)
+    end
 
   (* Generate a typable, closed random term. Rejection sampler with early abort
   that fails via exceptions. *)
@@ -74,9 +173,11 @@ ML \<open>
         ((s, (typ_env, maxidx)) : SpecCheck_Random.rand * (Type.tyenv * int))
         : (SpecCheck_Random.rand * (Type.tyenv * int)) * term =
     let
-      val (r, s) = range_real (0.0, 1.0) s
+      val (r, s) = SpecCheck_Generator.range_real (0.0, 1.0) s
     in
-      if boltzmann_index r
+      if boltzmann_constant r
+        then ran_constant ctxt typ (s, (typ_env, maxidx))
+      else if boltzmann_index r
         then pick_index ctxt binder_types typ (s, (typ_env, maxidx))
       else if boltzmann_lambda r
         then
@@ -113,9 +214,12 @@ ML \<open>
         end
     end
 
-  val boltzmann_term_failing_gen : (term, SpecCheck_Random.rand) gen_state = fn s =>
+  type boltzmann_config =
+    { T : typ, free_names : string list, const_names : string list, min_size : int }
+
+  fun boltzmann_term_of_type_failing_gen (T : typ) : (term, SpecCheck_Random.rand) SpecCheck_Generator.gen_state = fn s =>
     let
-      val (maxidx, T) = gen_fresh_tyvar @{context} ~1
+      val maxidx = Term.maxidx_of_typ T
       val ((s, (typ_env, maxidx)), t) =
         ran_typable @{context} [] T (s, (Vartab.empty, maxidx))
       val t =
@@ -125,6 +229,9 @@ ML \<open>
     in
       (t, s)
     end
+
+  val boltzmann_term_failing_gen =
+    boltzmann_term_of_type_failing_gen (snd (gen_fresh_tyvar @{context} 1))
 
   (* rejection sampling *)
   fun retry_on_exception_gen gen s =
@@ -137,22 +244,84 @@ ML \<open>
 
   val boltzmann_term_gen = retry_on_exception_gen boltzmann_term_failing_gen
 
-  fun boltzmann_term_gen_min_size min_size =
+  fun min_size_gen min_size gen =
     SpecCheck_Generator.filter
       (fn t => size_of_term t >= min_size)
-      boltzmann_term_gen
+      gen
+
+  fun boltzmann_term_gen_min_size min_size
+    = min_size_gen min_size boltzmann_term_gen
+  
+  fun boltzmann_term_of_type_gen T = retry_on_exception_gen (boltzmann_term_of_type_failing_gen T)
+
+\<close>
+
+declare [[speccheck_num_counterexamples = 10]]
+declare [[speccheck_max_success = 10]]
+
+(* declare [[show_types]] *)
+
+ML \<open>
+  (* val check_term = SpecCheck.check (SpecCheck_Show.term @{context}) (boltzmann_term_gen_min_size 0) *)
+  val check_term =
+    SpecCheck.check
+      (SpecCheck_Show.term @{context})
+      (
+        SpecCheck_Generator.map
+          (fn t => JTerm.ensure_lambda_under_q (HOLogic.all_const (body_type (fastype_of t)) $ t))
+          (min_size_gen 5 (boltzmann_term_of_type_gen @{typ_pat "(?'a => bool)"}))
+      )
+  val ctxt = Proof_Context.set_mode Proof_Context.mode_schematic @{context}
+  val _ = Lecker.test_group ctxt (SpecCheck_Random.new ()) [
+    SpecCheck_Property.prop (K false) (* (is_some o try (Syntax.check_term ctxt)) *)
+    |> check_term "boltzmann generator type checks"
+  ]
 \<close>
 
 declare [[speccheck_num_counterexamples = 10]]
 declare [[speccheck_max_success = 10]]
 
 ML \<open>
-  val check_term = check (SpecCheck_Show.term @{context}) (boltzmann_term_gen_min_size 10)
+  fun show_termpair ctxt =
+    let val pretty_term = Syntax.pretty_term ctxt
+    in SpecCheck_Show.zip pretty_term pretty_term end
+  val term_gen = boltzmann_term_gen_min_size 3
+  val boltzmann_term_pair_gen = SpecCheck_Generator.zip term_gen term_gen
   val ctxt = Proof_Context.set_mode Proof_Context.mode_schematic @{context}
+  val check_kbo = SpecCheck.check (show_termpair ctxt) boltzmann_term_pair_gen
+  (* print some unifiable terms lambda expressions *)
   val _ = Lecker.test_group ctxt (SpecCheck_Random.new ()) [
-    SpecCheck_Property.prop (is_some o try (Syntax.check_term ctxt))
-    |> check_term "boltzmann generator type checks"
+    SpecCheck_Property.prop (fn term_pair => (is_none o Seq.pull) ( Jeha_Unify.smash_unifiers (Context.Proof ctxt) [term_pair] Envir.init)) |> check_kbo "kbo"
   ]
+
+  (* val smash_unifiers: Context.generic -> (term * term) list -> Envir.env -> Envir.env Seq.seq *)
+\<close>
+
+declare [[show_types, show_sorts]]
+
+ML \<open>
+  val c = Sign.consts_of @{theory} |> Consts.dest |> #constraints;
+  val cs =
+    Sign.consts_of @{theory} |> Consts.dest |> #constants
+    |> filter (fn (name, _) => String.isPrefix "HOL" name andalso String.size name <= 11);
+  val pretty_cs =
+    cs
+    |> map (fn (name, (T, t)) =>
+        Pretty.block ([
+          Pretty.str (name ^ " : "),
+          Syntax.pretty_typ @{context} T
+        ]
+        @
+        (case t of
+          SOME t =>
+            [
+              Pretty.str "            (",
+              Syntax.pretty_term @{context} t,
+              Pretty.str ")"
+            ]
+        | NONE => []))
+        )
+    |> Pretty.enum "\n" "[" "]"
 \<close>
 
 end
